theories/logrel/ftlr_msg_send.v
@@ -11,8 +11,9 @@ Section ftlr_msg_send.
   Context `{hypparams:!HypervisorParameters}.
   Context `{vmG: !gen_VMG Σ}.
 
-  Lemma ftlr_msg_send {i mem_acc_tx ai regs ps_acc p_tx p_rx instr trans rx_state r0}:
+  Lemma ftlr_msg_send {i mem_acc_tx ai regs ps_acc p_tx p_rx instr trans rxs r0}:
     base_extra.is_total_gmap regs ->
+    base_extra.is_total_gmap rxs ->
     i ≠ V0 ->
     {[p_tx; p_rx]} ⊆ ps_acc ->
     currently_accessible_in_trans_memory_pages i trans ⊆ ps_acc ∖ {[p_tx; p_rx]} ->
@@ -28,7 +29,8 @@ Section ftlr_msg_send.
     regs !! R0 = Some r0 ->
     decode_hvc_func r0 = Some Send ->
     p_tx ≠ p_rx ->
-    ⊢ ▷ (∀ (a : gmap reg_name Addr) (a0 : gset PID) (a1 : gmap Addr transaction) (a2 : option (Addr * VMID)),
+  ⊢ ▷ (∀ (a : gmap reg_name Addr) (a0 : gset PID) (a1 : gmap Addr transaction) (a2 : gmap VMID (option (Addr * VMID))),
+              ⌜base_extra.is_total_gmap a2⌝ -∗
               ⌜base_extra.is_total_gmap a⌝ -∗
               ⌜{[p_tx; p_rx]} ⊆ a0⌝ -∗
               ⌜currently_accessible_in_trans_memory_pages i a1 ⊆ a0 ∖ {[p_tx; p_rx]}⌝ -∗
@@ -45,10 +47,10 @@ Section ftlr_msg_send.
               R0 @@ V0 ->r encode_hvc_func Run -∗
               R1 @@ V0 ->r encode_vmid i -∗
               (∃ r2 : Addr, R2 @@ V0 ->r r2) -∗
-              RX_state@i:= a2 -∗
               mailbox.rx_page i p_rx -∗
-              rx_pages (list_to_set list_of_vmids ∖ {[i]}) -∗
-              ▷ VMProp V0 (vmprop_zero i p_tx p_rx) (1 / 2) -∗
+              rx_state_get i a2 -∗
+              rx_states_global (delete i a2) -∗
+              ▷ VMProp V0 (vmprop_zero i p_tx p_rx a2) (1 / 2) -∗
               VMProp i (vmprop_unknown i p_tx p_rx) 1 -∗
               transaction_pagetable_entries_owned i a1 -∗
               retrieved_transaction_owned i a1 -∗
@@ -65,10 +67,10 @@ Section ftlr_msg_send.
    R0 @@ V0 ->r encode_hvc_func Run -∗
    R1 @@ V0 ->r encode_vmid i -∗
    (∃ r2 : Addr, R2 @@ V0 ->r r2) -∗
-   RX_state@i:= rx_state -∗
+   rx_state_get i rxs -∗
    mailbox.rx_page i p_rx -∗
-   rx_pages (list_to_set list_of_vmids ∖ {[i]}) -∗
-   ▷ VMProp V0 (vmprop_zero i p_tx p_rx) (1 / 2) -∗
+   rx_states_global (delete i rxs) -∗
+   ▷ VMProp V0 (vmprop_zero i p_tx p_rx rxs) (1 / 2) -∗
    VMProp i (vmprop_unknown i p_tx p_rx) 1 -∗
    transaction_pagetable_entries_owned i trans -∗
    retrieved_transaction_owned i trans -∗
@@ -77,9 +79,9 @@ Section ftlr_msg_send.
    (∃ mem2 : mem, memory_page p_tx mem2) -∗
    SSWP ExecI @ i {{ bm, (if bm.1 then VMProp_holds i (1 / 2) else True) -∗ WP bm.2 @ i {{ _, True }} }}.
   Proof.
-    iIntros (Htotal_regs Hneq_0 Hsubset_mb Hsubset_acc Hnin_rx Hnin_tx Hlookup_PC Hin_ps_acc Hneq_ptx Hdom_mem_acc_tx Hin_ps_acc_tx
-                         Hlookup_mem_ai Heqn  Hlookup_reg_R0 Hdecode_hvc).
-    iIntros (Hneq_mb) "IH regs tx pgt_tx pgt_acc pgt_owned trans_hpool_global tran_pgt_transferred retri R0z R1z R2z rx_state rx other_rx prop0
+    iIntros (Htotal_regs Htotal_rxs Hneq_0 Hsubset_mb Hsubset_acc Hnin_rx Hnin_tx Hlookup_PC Hin_ps_acc Hneq_ptx Hdom_mem_acc_tx Hin_ps_acc_tx
+                         Hlookup_mem_ai Heqn  Hlookup_reg_R0 ).
+    iIntros (Hdecode_hvc Hneq_mb) "IH regs tx pgt_tx pgt_acc pgt_owned trans_hpool_global tran_pgt_transferred retri R0z R1z R2z rx_state rx other_rx prop0
              propi tran_pgt_owned retri_owned mem_rest mem_acc_tx mem_tx".
     set ps_mem_in_trans := accessible_in_trans_memory_pages i trans.
     pose proof (Htotal_regs R1) as[r1 Hlookup_reg_R1].
@@ -95,8 +97,8 @@ Section ftlr_msg_send.
       iDestruct ("Hacc_regs" $! (ai ^+ 1)%f with "[$ PC $ R0 $ R1 $ R2]") as (regs') "[%Htotal_regs' regs]".
 
       iDestruct ("Hacc_mem_acc_tx" with "[$mem_instr]") as "mem_acc_tx".
-      iApply ("IH" $! _ ps_acc trans _ Htotal_regs' Hsubset_mb Hsubset_acc Hnin_rx Hnin_tx with "regs tx pgt_tx pgt_acc pgt_owned trans_hpool_global
-                            tran_pgt_transferred retri R0z R1z R2z rx_state rx other_rx prop0 propi tran_pgt_owned retri_owned [mem_rest mem_acc_tx mem_tx]
+      iApply ("IH" $! _ ps_acc trans _ Htotal_rxs Htotal_regs' Hsubset_mb Hsubset_acc Hnin_rx Hnin_tx with "regs tx pgt_tx pgt_acc pgt_owned trans_hpool_global
+                            tran_pgt_transferred retri R0z R1z R2z rx rx_state other_rx prop0 propi tran_pgt_owned retri_owned [mem_rest mem_acc_tx mem_tx]
                             ").
       {
         iDestruct (memory_pages_split_singleton' p_tx ps_acc with "[mem_acc_tx $mem_tx]") as "mem_acc". set_solver + Hsubset_mb.
@@ -114,8 +116,8 @@ Section ftlr_msg_send.
       iDestruct ("Hacc_regs" $! (ai ^+ 1)%f with "[$ PC $ R0 $ R1 $ R2]") as (regs') "[%Htotal_regs' regs]".
 
       iDestruct ("Hacc_mem_acc_tx" with "[$mem_instr]") as "mem_acc_tx".
-      iApply ("IH" $! _ ps_acc trans _ Htotal_regs' Hsubset_mb Hsubset_acc Hnin_rx Hnin_tx with "regs tx pgt_tx pgt_acc pgt_owned trans_hpool_global
-                            tran_pgt_transferred retri R0z R1z R2z rx_state rx other_rx prop0 propi tran_pgt_owned retri_owned [mem_rest mem_acc_tx mem_tx]
+      iApply ("IH" $! _ ps_acc trans _ Htotal_rxs Htotal_regs' Hsubset_mb Hsubset_acc Hnin_rx Hnin_tx with "regs tx pgt_tx pgt_acc pgt_owned trans_hpool_global
+                            tran_pgt_transferred retri R0z R1z R2z rx rx_state other_rx prop0 propi tran_pgt_owned retri_owned [mem_rest mem_acc_tx mem_tx]
                             ").
       {
         iDestruct (memory_pages_split_singleton' p_tx ps_acc with "[mem_acc_tx $mem_tx]") as "mem_acc". set_solver + Hsubset_mb.
@@ -133,8 +135,8 @@ Section ftlr_msg_send.
       iDestruct ("Hacc_regs" $! (ai ^+ 1)%f with "[$ PC $ R0 $ R1 $ R2]") as (regs') "[%Htotal_regs' regs]".
 
       iDestruct ("Hacc_mem_acc_tx" with "[$mem_instr]") as "mem_acc_tx".
-      iApply ("IH" $! _ ps_acc trans _ Htotal_regs' Hsubset_mb Hsubset_acc Hnin_rx Hnin_tx with "regs tx pgt_tx pgt_acc pgt_owned trans_hpool_global
-                            tran_pgt_transferred retri R0z R1z R2z rx_state rx other_rx prop0 propi tran_pgt_owned retri_owned [mem_rest mem_acc_tx mem_tx]
+      iApply ("IH" $! _ ps_acc trans _ Htotal_rxs Htotal_regs' Hsubset_mb Hsubset_acc Hnin_rx Hnin_tx with "regs tx pgt_tx pgt_acc pgt_owned trans_hpool_global
+                            tran_pgt_transferred retri R0z R1z R2z rx rx_state other_rx prop0 propi tran_pgt_owned retri_owned [mem_rest mem_acc_tx mem_tx]
                             ").
       {
         iDestruct (memory_pages_split_singleton' p_tx ps_acc with "[mem_acc_tx $mem_tx]") as "mem_acc". set_solver + Hsubset_mb.
@@ -144,35 +146,34 @@ Section ftlr_msg_send.
       }
     }
 
-    set all_vmids := (list_to_set (list_of_vmids)).
-    assert (v ∈ (all_vmids ∖ {[i]})) as Hin_v.
+    assert (is_Some((delete i rxs)!! v)) as Hin_v.
     {
-      pose proof (in_list_of_vmids v) as Hin_v.
-      rewrite -elem_of_list_In in Hin_v.
-      rewrite -(elem_of_list_to_set (C:= gset _)) in Hin_v.
-      set_solver + Hin_v n.
+      pose proof (Htotal_rxs v) as [? ?].
+      exists x.
+      rewrite lookup_delete_ne //.
     }
 
-    iDestruct (big_sepS_delete with "other_rx") as "[(%p_rx_v & [rx_v [%rx_state_v [rx_state_v rx_state_v']]]) other_rx]".
+    destruct Hin_v as [rx_state_v Hin_v].
+    iDestruct (big_sepM_delete with "other_rx") as "[rx_state_v other_rx]".
     exact Hin_v.
 
     destruct (rx_state_v).
     { (* apply [msg_send_full_rx] *)
+      iEval (rewrite /rx_state_match /= /rx_state_some) in "rx_state_v".
       iApply (msg_send_full_rx ai with "[PC mem_instr pgt_acc R0 R1 R2 tx rx_state_v]");iFrameAutoSolve.
-      exact Heq_decode. done. lia. 2: { iFrame "rx_state_v". } done.
+      exact Heq_decode. done. lia. 2: { iDestruct "rx_state_v" as "[$ ?]". done. } done.
       iNext. iIntros "(PC & mem_instr & pgt_acc  & tx & R0 & R1 & R2 & rx_state_v ) _".
       iDestruct ("Hacc_regs" $! (ai ^+ 1)%f with "[$ PC $ R0 $ R1 $ R2]") as (regs') "[%Htotal_regs' regs]".
 
       iDestruct ("Hacc_mem_acc_tx" with "[$mem_instr]") as "mem_acc_tx".
-      iApply ("IH" $! _ ps_acc trans _ Htotal_regs' Hsubset_mb Hsubset_acc Hnin_rx Hnin_tx with "regs tx pgt_tx pgt_acc pgt_owned trans_hpool_global
-                            tran_pgt_transferred retri R0z R1z R2z rx_state rx [other_rx rx_v rx_state_v rx_state_v'] prop0 propi tran_pgt_owned retri_owned [mem_rest mem_acc_tx mem_tx]
+      iApply ("IH" $! _ ps_acc trans _ Htotal_rxs Htotal_regs' Hsubset_mb Hsubset_acc Hnin_rx Hnin_tx with "regs tx pgt_tx pgt_acc pgt_owned trans_hpool_global
+                            tran_pgt_transferred retri R0z R1z R2z rx rx_state [other_rx rx_state_v] prop0 propi tran_pgt_owned retri_owned [mem_rest mem_acc_tx mem_tx]
                             ").
       {
-        iApply (big_sepS_delete with "[other_rx rx_v rx_state_v rx_state_v']").
+        iApply (big_sepM_delete with "[other_rx rx_state_v]").
         exact Hin_v.
         simpl. iFrame "other_rx".
-        iExists p_rx_v. iFrame.
-        iExists (Some p). iFrame.
+        iFrame.
       }
       {
         iDestruct (memory_pages_split_singleton' p_tx ps_acc with "[mem_acc_tx $mem_tx]") as "mem_acc". set_solver + Hsubset_mb.
@@ -181,8 +182,6 @@ Section ftlr_msg_send.
         set_solver +.
       }
     }
-    iDestruct ("rx_state_v'" with "[]") as "[rx_state_v' [%mem_rx_v mem_rx_v]]";auto.
-    iDestruct (rx_state_split with "[$rx_state_v $rx_state_v']") as "rx_state_v".
 
     iDestruct ("Hacc_mem_acc_tx" with "[$mem_instr]") as "mem_acc_tx".
     pose proof (union_split_difference_intersection_L (ps_acc∖ {[p_tx]}) ({[p_rx]} ∪ (transferred_memory_pages i trans))) as [Heq_ps_acc_tx Hdisj_ps_acc_tx].
@@ -259,12 +258,14 @@ Section ftlr_msg_send.
       { set_solver +. }
       rewrite Heq_inter_diff_union.
 
+      iDestruct "rx_state_v" as "[rx_state_v [%p_rx_v [rx_v [%mem_rx_v mem_rx_v]]]]".
+
       (* getting instruction from [mem_oea] *)
       iDestruct (mem_big_sepM_split mem_oea Hlookup_mem_ai' with "mem_oea") as "[mem_instr Hacc_mem]".
       iApply (msg_send_secondary ai v (transaction_hpool_global_transferred trans ∗
                                                          transaction_pagetable_entries_transferred i trans ∗
                                                          retrievable_transaction_transferred i trans ∗
-                                                         rx_pages (all_vmids ∖ {[i;v]}))%I _
+                                                         rx_states_global (delete v (delete i rxs)) )%I _
                with "[PC R0 R1 R2 R0z R1z R2z pgt_acc tx mem_tx mem_instr rx_v rx_state_v mem_rx_v other_rx prop0 propi
                     trans_hpool_global tran_pgt_transferred mem_tran retri rx_state rx]"); iFrameAutoSolve.
       { solve_finz + n0. }
@@ -274,14 +275,11 @@ Section ftlr_msg_send.
         iSplitL "mem_tx". iFrame "mem_tx".
         iSplitL "mem_rx_v". iFrame "mem_rx_v".
         iSplitR "trans_hpool_global tran_pgt_transferred retri other_rx".
-        2: {
-          iFrame.
-          rewrite /rx_pages difference_difference_L. iFrame.
-        }
+        2: { iFrame. }
         iNext. iIntros "((PC & mem_instr & pgt_acc & R0 & R1 & R2 & R0z & R1z & R2z & tx & #rx_v
                 & rx_state_v & mem_tx & [% (_ & _ & mem_rx_v)])
                 & (trans_hpool_global & trans_pgt_transferred & retri & other_rx) & propi)".
-        iSplitL "trans_hpool_global trans_pgt_transferred retri R0z R1z R2z rx_state rx other_rx mem_tran mem_rx_v rx_v rx_state_v propi".
+        iSplitL "trans_hpool_global trans_pgt_transferred retri R0z R1z R2z rx rx_state other_rx mem_tran mem_rx_v rx_v rx_state_v propi".
         iExists trans. iFrame "trans_hpool_global trans_pgt_transferred retri rx".
         (* split [mem_tran] into [mem_rx] and [mem_trans] *)
         iDestruct (memory_pages_split_union' with "mem_tran") as "[mem_rx mem_trans]".
@@ -291,20 +289,21 @@ Section ftlr_msg_send.
         rewrite memory_pages_singleton'.
         iFrame "mem_rx mem_trans".
         iDestruct (rx_state_split with "rx_state_v") as "[rx_state_v rx_state_v']".
-        iSplitL "other_rx rx_state_v".
-        iApply (big_sepS_delete _ _ v with "[rx_v rx_state_v other_rx]");auto.
-        simpl. rewrite difference_difference_L.
-        iFrame "other_rx".
-        iExists p_rx_v. iFrame "rx_v".
-        iExists (Some (r2, i)). iFrame.
-        iIntros "%". done.
+        pose proof (Htotal_rxs i) as [rs Hlookup_rs].
+        iExists rs. iSplitL "rx_state".
+        iDestruct ("rx_state" $! rs with "[]") as "rx_state".
+        done. iFrame.
         iSplitR "propi".
         iRight. iFrame "R0z".
-        iSplitL "rx_state". iExists rx_state. iFrame.
-        iExists v, p_rx_v, r2. iFrame.
-        iSplitL "";auto. iFrame "rx_v".
-        iSplitL "R1z". iExists r1. iFrame. done.
-        iExists (list_to_map (zip (finz.seq p_rx_v (length des)) des) ∪ mem_rx_v). iFrame.
+        iExists r2, v, p_rx_v.
+        iFrame "rx_v".
+        iFrame. iExists (list_to_map (zip (finz.seq p_rx_v (length des)) des) ∪ mem_rx_v). iFrame.
+        iSplitR "R1z".
+        iApply (big_sepM_delete _ _ v with "[rx_v rx_state_v other_rx]");auto.
+        rewrite lookup_insert. reflexivity.
+        rewrite delete_insert_delete.
+        simpl. iFrame.
+        iExists r1. iFrame. done.
         iExact "propi".
         iCombine "PC mem_instr R0 R1 R2 pgt_acc tx mem_tx" as "R'". iExact "R'".
       }
@@ -316,7 +315,7 @@ Section ftlr_msg_send.
       iEval (rewrite later_exist) in "Hres". iDestruct "Hres" as (rx_state') "Hres".
       iEval (rewrite 11!later_sep) in "Hres".
       iDestruct "Hres" as "(>trans_hpool_global & >tran_pgt_transferred &
-                         >retri & >mem_transferred & >R0z & >R1z & >R2z & >rx_state & >rx & >[% mem_rx] & >other_rx & prop0)".
+                         >retri & >mem_transferred & >R0z & >R1z & >R2z & >rx & >rx_state & >[% mem_rx] & >other_rx & >%Htotal_rxs' & prop0)".
       iDestruct ("Hacc_regs" $! (ai ^+ 1)%f r0 r1 r2 with "[PC R0 R1 R2]") as "[%regs' [%Htotal_regs' regs'']]"; iFrameAutoSolve.
       iDestruct (get_trans_rel_secondary with "[$trans_hpool_global $retri $tran_pgt_owned $retri_owned]") as "%trans_rel".
       erewrite (trans_rel_secondary_currently_accessible_memory_pages);eauto.
@@ -382,8 +381,8 @@ Section ftlr_msg_send.
         iExists mem_rx, mem2. rewrite 2!memory_pages_singleton. iFrame "mem_rx mem_tx". done.
         iPureIntro. rewrite map_union_assoc //. set_solver + Hneq_tx_rx.
       }
-      iApply ("IH" $! _ ps_acc trans' _ Htotal_regs' Hsubset_mb Hsubset_acc Hnin_rx' Hnin_tx' with "regs'' tx pgt_tx pgt_acc pgt_owned
-                        trans_hpool_global tran_pgt_transferred retri R0z R1z R2z rx_state rx other_rx prop0 propi
+      iApply ("IH" $! _ ps_acc trans' _ Htotal_rxs' Htotal_regs' Hsubset_mb Hsubset_acc Hnin_rx' Hnin_tx' with "regs'' tx pgt_tx pgt_acc pgt_owned
+                        trans_hpool_global tran_pgt_transferred retri R0z R1z R2z rx rx_state other_rx prop0 propi
                            tran_pgt_owned retri_owned mem").
     }
     { (* tpa ai ∉ ps_acc ∖ ({[p_rx]} ∪ ps_mem_in_trans) *)
@@ -409,8 +408,11 @@ Section ftlr_msg_send.
 
       (* get instruction *)
       iDestruct (mem_big_sepM_split mem_inters Hlookup_mem_ai' with "mem_inters") as "[mem_instr Hacc_mem_inters]".
+
+      iDestruct "rx_state_v" as "[rx_state_v [%p_rx_v [rx_v [%mem_rx_v mem_rx_v]]]]".
+
       iApply (msg_send_secondary ai v (transaction_hpool_global_transferred trans ∗ transaction_pagetable_entries_transferred i trans
-                                       ∗ retrievable_transaction_transferred i trans ∗ rx_pages (all_vmids ∖ {[i;v]})) _
+                                       ∗ retrievable_transaction_transferred i trans ∗ rx_states_global (delete v (delete i rxs))) _
                with "[PC R0 R1 R2 R0z R1z R2z pgt_acc tx mem_tx mem_instr rx_v rx_state_v mem_rx_v other_rx prop0 propi
                     trans_hpool_global tran_pgt_transferred Hacc_mem_inters mem_rest retri rx_state rx]"); iFrameAutoSolve.
       { solve_finz + n0. }
@@ -420,10 +422,7 @@ Section ftlr_msg_send.
         iSplitL "mem_tx". iFrame "mem_tx".
         iSplitL "mem_rx_v". iFrame "mem_rx_v".
         iSplitR "trans_hpool_global tran_pgt_transferred retri other_rx".
-        2: {
-          iFrame.
-          rewrite /rx_pages. rewrite difference_difference_L. iFrame.
-        }
+        2: { iFrame. }
         iNext. iIntros "((PC & mem_instr & pgt_acc & R0 & R1 & R2 & R0z & R1z & R2z & tx & #rx_v
                 & rx_state_v & mem_tx & [% (_ & _ & mem_rx_v)]) & (trans_hpool_global & trans_pgt_transferred & retri& other_rx) & propi)".
         iDestruct ("Hacc_mem_inters" with "mem_instr") as "mem_inters".
@@ -436,7 +435,7 @@ Section ftlr_msg_send.
         2:{ iSplitL "mem_inters". iExists mem_inters. iFrame "mem_inters". iExact "mem_rest". }
         { set_solver +. }
         rewrite Heq_inter_diff_union.
-        iSplitL "trans_hpool_global trans_pgt_transferred retri R0z R1z R2z rx_state rx other_rx mem_tran rx_v rx_state_v mem_rx_v propi".
+        iSplitL "trans_hpool_global trans_pgt_transferred retri R0z R1z R2z rx rx_state other_rx mem_tran rx_v rx_state_v mem_rx_v propi".
         iExists trans. iFrame "trans_hpool_global trans_pgt_transferred retri rx".
         iDestruct (memory_pages_split_union' with "mem_tran") as "[mem1 mem2]".
         { pose proof (transferred_accessible_memory_pages_subseteq i trans) as Hs.
@@ -445,18 +444,21 @@ Section ftlr_msg_send.
         iFrame "mem2".
         rewrite memory_pages_singleton'. iFrame "mem1".
         iDestruct (rx_state_split with "rx_state_v") as "[rx_state_v rx_state_v']".
-        iSplitL "other_rx rx_v rx_state_v".
-        iApply (big_sepS_delete _ _ v with "[rx_v rx_state_v other_rx]");auto.
-        simpl. rewrite difference_difference_L. iFrame "other_rx".
-        iExists p_rx_v. iFrame "rx_v".
-        iExists (Some (r2, i)). iFrame.
-        iIntros "%". done.
-        iSplitR "propi". iRight. iFrame.
-        iSplitL "rx_state". iExists rx_state. iFrame.
-        iExists v, p_rx_v, r2. iFrame.
-        iSplitL "";auto. iFrame "rx_v".
-        iSplitL "R1z". iExists r1. iFrame. done.
-        iExists (list_to_map (zip (finz.seq p_rx_v (length des)) des) ∪ mem_rx_v). iFrame.
+        pose proof (Htotal_rxs i) as [rs Hlookup_rs].
+        iExists rs. iSplitL "rx_state".
+        iDestruct ("rx_state" $! rs with "[]") as "rx_state".
+        done. iFrame.
+        iSplitR "propi".
+        iRight. iFrame "R0z".
+        iExists r2, v, p_rx_v.
+        iFrame "rx_v".
+        iFrame. iExists (list_to_map (zip (finz.seq p_rx_v (length des)) des) ∪ mem_rx_v). iFrame.
+        iSplitR "R1z".
+        iApply (big_sepM_delete _ _ v with "[rx_v rx_state_v other_rx]");auto.
+        rewrite lookup_insert. reflexivity.
+        rewrite delete_insert_delete.
+        simpl. iFrame.
+        iExists r1. iFrame. done.
         iExact "propi".
         iCombine "PC R0 R1 R2 pgt_acc tx mem_tx" as "R'". iExact "R'".
       }
@@ -468,7 +470,7 @@ Section ftlr_msg_send.
       iEval (rewrite later_exist) in "Hres". iDestruct "Hres" as (rx_state') "Hres".
       iEval (rewrite 11!later_sep) in "Hres".
       iDestruct "Hres" as "(>trans_hpool_global & >tran_pgt_transferred &
-                         >retri & >mem_transferred & >R0z & >R1z & >R2z & >rx_state & >rx & >[% mem_rx] & >other_rx & prop0)".
+                         >retri & >mem_transferred & >R0z & >R1z & >R2z & >rx & >rx_state & >[% mem_rx] & >other_rx & >%Htotal_rxs' & prop0)".
       iDestruct ("Hacc_regs" $! (ai ^+ 1)%f r0 r1 r2 with "[PC R0 R1 R2]") as "[%regs' [%Htotal_regs' regs'']]"; iFrameAutoSolve.
       iDestruct (get_trans_rel_secondary with "[$trans_hpool_global $retri $tran_pgt_owned $retri_owned]") as "%trans_rel".
       erewrite (trans_rel_secondary_currently_accessible_memory_pages);eauto.
@@ -532,8 +534,8 @@ Section ftlr_msg_send.
         done.
         iPureIntro. rewrite map_union_assoc //. set_solver + Hneq_tx_rx.
       }
-      iApply ("IH" $! _ ps_acc trans' _ Htotal_regs' Hsubset_mb Hsubset_acc Hnin_rx' Hnin_tx' with "regs'' tx pgt_tx pgt_acc pgt_owned
-                        trans_hpool_global tran_pgt_transferred retri R0z R1z R2z rx_state rx other_rx prop0 propi
+      iApply ("IH" $! _ ps_acc trans' _ Htotal_rxs' Htotal_regs' Hsubset_mb Hsubset_acc Hnin_rx' Hnin_tx' with "regs'' tx pgt_tx pgt_acc pgt_owned
+                        trans_hpool_global tran_pgt_transferred retri R0z R1z R2z rx rx_state other_rx prop0 propi
                            tran_pgt_owned retri_owned mem").
     }
   Qed.
