theories/logrel/ftlr_reclaim.v
@@ -12,8 +12,9 @@ Section ftlr_reclaim.
   Context `{hypparams:!HypervisorParameters}.
   Context `{vmG: !gen_VMG Σ}.
 
-Lemma ftlr_reclaim {i mem_acc_tx ai regs ps_acc p_tx p_rx instr trans rx_state r0}:
+Lemma ftlr_reclaim {i mem_acc_tx ai regs ps_acc p_tx p_rx instr trans rxs r0}:
   base_extra.is_total_gmap regs ->
+  base_extra.is_total_gmap rxs ->
   {[p_tx; p_rx]} ⊆ ps_acc ->
   currently_accessible_in_trans_memory_pages i trans ⊆ ps_acc ∖ {[p_tx; p_rx]} ->
   p_rx ∉ ps_acc ∖ {[p_rx; p_tx]} ∪ accessible_in_trans_memory_pages i trans ->
@@ -28,7 +29,8 @@ Lemma ftlr_reclaim {i mem_acc_tx ai regs ps_acc p_tx p_rx instr trans rx_state r
   regs !! R0 = Some r0 ->
   decode_hvc_func r0 = Some Reclaim ->
   p_tx ≠ p_rx ->
-  ⊢ ▷ (∀ (a : gmap reg_name Addr) (a0 : gset PID) (a1 : gmap Addr transaction) (a2 : option (Addr * VMID)),
+  ⊢ ▷ (∀ (a : gmap reg_name Addr) (a0 : gset PID) (a1 : gmap Addr transaction) (a2 : gmap VMID (option (Addr * VMID))),
+              ⌜base_extra.is_total_gmap a2⌝ -∗
               ⌜base_extra.is_total_gmap a⌝ -∗
               ⌜{[p_tx; p_rx]} ⊆ a0⌝ -∗
               ⌜currently_accessible_in_trans_memory_pages i a1 ⊆ a0 ∖ {[p_tx; p_rx]}⌝ -∗
@@ -45,10 +47,10 @@ Lemma ftlr_reclaim {i mem_acc_tx ai regs ps_acc p_tx p_rx instr trans rx_state r
               R0 @@ V0 ->r encode_hvc_func Run -∗
               R1 @@ V0 ->r encode_vmid i -∗
               (∃ r2 : Addr, R2 @@ V0 ->r r2) -∗
-              RX_state@i:= a2 -∗
               mailbox.rx_page i p_rx -∗
-              rx_pages (list_to_set list_of_vmids ∖ {[i]}) -∗
-              ▷ VMProp V0 (vmprop_zero i p_tx p_rx) (1 / 2) -∗
+              rx_state_get i a2 -∗
+              rx_states_global (delete i a2) -∗
+              ▷ VMProp V0 (vmprop_zero i p_tx p_rx a2) (1 / 2) -∗
               VMProp i (vmprop_unknown i p_tx p_rx) 1 -∗
               transaction_pagetable_entries_owned i a1 -∗
               retrieved_transaction_owned i a1 -∗
@@ -65,10 +67,10 @@ Lemma ftlr_reclaim {i mem_acc_tx ai regs ps_acc p_tx p_rx instr trans rx_state r
    R0 @@ V0 ->r encode_hvc_func Run -∗
    R1 @@ V0 ->r encode_vmid i -∗
    (∃ r2 : Addr, R2 @@ V0 ->r r2) -∗
-   RX_state@i:= rx_state -∗
+   rx_state_get i rxs -∗
    mailbox.rx_page i p_rx -∗
-   rx_pages (list_to_set list_of_vmids ∖ {[i]}) -∗
-   ▷ VMProp V0 (vmprop_zero i p_tx p_rx) (1 / 2) -∗
+   rx_states_global (delete i rxs) -∗
+   ▷ VMProp V0 (vmprop_zero i p_tx p_rx rxs) (1 / 2) -∗
    VMProp i (vmprop_unknown i p_tx p_rx) 1 -∗
    transaction_pagetable_entries_owned i trans -∗
    retrieved_transaction_owned i trans -∗
@@ -77,9 +79,9 @@ Lemma ftlr_reclaim {i mem_acc_tx ai regs ps_acc p_tx p_rx instr trans rx_state r
    (∃ mem2 : mem, memory_page p_tx mem2) -∗
    SSWP ExecI @ i {{ bm, (if bm.1 then VMProp_holds i (1 / 2) else True) -∗ WP bm.2 @ i {{ _, True }} }}.
   Proof.
-    iIntros (Htotal_regs Hsubset_mb Hsubset_acc Hnin_rx Hnin_tx Hlookup_PC Hin_ps_acc Hneq_ptx Hdom_mem_acc_tx Hin_ps_acc_tx
-                         Hlookup_mem_ai Heqn Hlookup_reg_R0 Hdecode_hvc Hneq_mb).
-    iIntros "IH regs tx pgt_tx pgt_acc pgt_owned trans_hpool_global tran_pgt_transferred retri R0z R1z R2z rx_state rx other_rx prop0
+    iIntros (Htotal_regs Htotal_rxs Hsubset_mb Hsubset_acc Hnin_rx Hnin_tx Hlookup_PC Hin_ps_acc Hneq_ptx Hdom_mem_acc_tx Hin_ps_acc_tx
+                         Hlookup_mem_ai Heqn Hlookup_reg_R0 Hdecode_hvc).
+    iIntros (Hneq_mb) "IH regs tx pgt_tx pgt_acc pgt_owned trans_hpool_global tran_pgt_transferred retri R0z R1z R2z rx_state rx other_rx prop0
              propi tran_pgt_owned retri_owned mem_rest mem_acc_tx mem_tx".
     set ps_mem_in_trans := accessible_in_trans_memory_pages i trans.
     pose proof (Htotal_regs R1) as[r1 Hlookup_reg_R1].
@@ -99,8 +101,8 @@ Lemma ftlr_reclaim {i mem_acc_tx ai regs ps_acc p_tx p_rx instr trans rx_state r
       iDestruct ("Hacc_regs" $! (ai ^+ 1)%f with "[$ PC $ R0 $ R1 $ R2]") as (regs') "[%Htotal_regs' regs]".
       iDestruct ("Hacc_mem_acc_tx" with "[$mem_instr]") as "mem_acc_tx".
 
-      iApply ("IH" $! _ _ trans _ Htotal_regs' with "[] [] [] [] regs tx pgt_tx pgt_acc pgt_owned [fresh_handles trans]
-                            tran_pgt_transferred retri R0z R1z R2z rx_state rx other_rx prop0 propi tran_pgt_owned
+      iApply ("IH" $! _ _ trans _ Htotal_rxs Htotal_regs' with "[] [] [] [] regs tx pgt_tx pgt_acc pgt_owned [fresh_handles trans]
+                            tran_pgt_transferred retri R0z R1z R2z rx rx_state other_rx prop0 propi tran_pgt_owned
                              retri_owned [mem_rest mem_acc_tx mem_tx]");auto.
       {
         iExists hpool.
@@ -123,8 +125,8 @@ Lemma ftlr_reclaim {i mem_acc_tx ai regs ps_acc p_tx p_rx instr trans rx_state r
       iDestruct ("Hacc_regs" $! (ai ^+ 1)%f with "[$ PC $ R0 $ R1 $ R2]") as (regs') "[%Htotal_regs' regs]".
       iDestruct ("Hacc_mem_acc_tx" with "[$mem_instr]") as "mem_acc_tx".
 
-      iApply ("IH" $! _ _ trans _ Htotal_regs' with "[] [] [] [] regs tx pgt_tx pgt_acc pgt_owned [fresh_handles trans]
-                            tran_pgt_transferred retri R0z R1z R2z rx_state rx other_rx prop0 propi tran_pgt_owned
+      iApply ("IH" $! _ _ trans _ Htotal_rxs Htotal_regs' with "[] [] [] [] regs tx pgt_tx pgt_acc pgt_owned [fresh_handles trans]
+                            tran_pgt_transferred retri R0z R1z R2z rx rx_state other_rx prop0 propi tran_pgt_owned
                             retri_owned [mem_rest mem_acc_tx mem_tx]");auto.
       {
         iExists hpool.
@@ -157,8 +159,8 @@ Lemma ftlr_reclaim {i mem_acc_tx ai regs ps_acc p_tx p_rx instr trans rx_state r
       iDestruct ("Hacc_regs" $! (ai ^+ 1)%f with "[$ PC $ R0 $ R1 $ R2]") as (regs') "[%Htotal_regs' regs]".
       iDestruct ("Hacc_mem_acc_tx" with "[$mem_instr]") as "mem_acc_tx".
 
-      iApply ("IH" $! _ _ trans _ Htotal_regs' with "[] [] [] [] regs tx pgt_tx pgt_acc pgt_owned [fresh_handles tran pgt_tran trans]
-                            tran_pgt_transferred retri R0z R1z R2z rx_state rx other_rx prop0 propi tran_pgt_owned
+      iApply ("IH" $! _ _ trans _ Htotal_rxs Htotal_regs' with "[] [] [] [] regs tx pgt_tx pgt_acc pgt_owned [fresh_handles tran pgt_tran trans]
+                            tran_pgt_transferred retri R0z R1z R2z rx rx_state other_rx prop0 propi tran_pgt_owned
                             retri_owned [mem_rest mem_acc_tx mem_tx]");auto.
       {
         iExists hpool.
@@ -177,7 +179,7 @@ Lemma ftlr_reclaim {i mem_acc_tx ai regs ps_acc p_tx p_rx instr trans rx_state r
 
     iDestruct ("retri") as "[retri retri']".
     iDestruct (big_sepFM_lookup_Some Hlookup_tran with "retri") as "[re retri]".
-    simpl;right;done.
+    left;done.
 
     destruct (tran.2) eqn:Heq_retri.
     { (* apply [mem_reclaim_retrieved] *)
@@ -189,8 +191,8 @@ Lemma ftlr_reclaim {i mem_acc_tx ai regs ps_acc p_tx p_rx instr trans rx_state r
       iDestruct ("Hacc_regs" $! (ai ^+ 1)%f with "[$ PC $ R0 $ R1 $ R2]") as (regs') "[%Htotal_regs' regs]".
       iDestruct ("Hacc_mem_acc_tx" with "[$mem_instr]") as "mem_acc_tx".
 
-      iApply ("IH" $! _ _ trans _ Htotal_regs' with "[] [] [] [] regs tx pgt_tx pgt_acc pgt_owned [fresh_handles tran pgt_tran trans]
-                            tran_pgt_transferred [re retri retri'] R0z R1z R2z rx_state rx other_rx prop0 propi tran_pgt_owned
+      iApply ("IH" $! _ _ trans _ Htotal_rxs Htotal_regs' with "[] [] [] [] regs tx pgt_tx pgt_acc pgt_owned [fresh_handles tran pgt_tran trans]
+                            tran_pgt_transferred [re retri retri'] R0z R1z R2z rx rx_state other_rx prop0 propi tran_pgt_owned
                             retri_owned [mem_rest mem_acc_tx mem_tx]");auto.
       {
         iExists hpool.
@@ -202,7 +204,7 @@ Lemma ftlr_reclaim {i mem_acc_tx ai regs ps_acc p_tx p_rx instr trans rx_state r
       {
         rewrite /retrievable_transaction_transferred.
         iDestruct (big_sepFM_delete_acc_True tran with "retri") as "retri".
-        simpl. right;done.
+        left;done.
         rewrite Heq_retri.
         iDestruct ("retri" with "re") as "retri".
         rewrite insert_id;auto.
@@ -261,7 +263,7 @@ Lemma ftlr_reclaim {i mem_acc_tx ai regs ps_acc p_tx p_rx instr trans rx_state r
     { (* apply [mem_reclaim_donate] *)
     iDestruct (mem_big_sepM_split mem_acc_tx Hlookup_mem_ai with "mem_acc_tx") as "[mem_instr Hacc_mem_acc_tx]".
     iDestruct (big_sepFM_lookup_Some Hlookup_tran with "tran_pgt_transferred") as "[[tran' oe_tran] tran_pgt_transferred]".
-    simpl. split;first done. eauto.
+    simpl. split;last done. eauto.
     rewrite Hrw_tran; clear Hrw_tran.
 
     iDestruct (trans_split with "[tran' tran'']") as "tran'".
@@ -274,9 +276,9 @@ Lemma ftlr_reclaim {i mem_acc_tx ai regs ps_acc p_tx p_rx instr trans rx_state r
     iDestruct ("Hacc_regs" $! (ai ^+ 1)%f with "[$ PC $ R0 $ R1 $ R2]") as (regs') "[%Htotal_regs' regs]".
     iDestruct ("Hacc_mem_acc_tx" with "[$mem_instr]") as "mem_acc_tx".
 
-    iApply ("IH" $! _ _ (delete r1 trans) _ Htotal_regs' with "[] [] [] [] regs tx pgt_tx pgt_acc [oe_tran pgt_tran pgt_owned]
+    iApply ("IH" $! _ _ (delete r1 trans) _ Htotal_rxs Htotal_regs' with "[] [] [] [] regs tx pgt_tx pgt_acc [oe_tran pgt_tran pgt_owned]
                             [fresh_handles trans]
-                            [tran_pgt_transferred] [retri retri'] R0z R1z R2z rx_state rx other_rx prop0 propi [tran_pgt_owned]
+                            [tran_pgt_transferred] [retri retri'] R0z R1z R2z rx rx_state other_rx prop0 propi [tran_pgt_owned]
                              [retri_owned] [mem_rest mem_acc_tx mem_tx]").
     {
       iPureIntro.
@@ -395,8 +397,8 @@ Lemma ftlr_reclaim {i mem_acc_tx ai regs ps_acc p_tx p_rx instr trans rx_state r
     iDestruct ("Hacc_regs" $! (ai ^+ 1)%f with "[$ PC $ R0 $ R1 $ R2]") as (regs') "[%Htotal_regs' regs]".
     iDestruct ("Hacc_mem_acc_tx" with "[$mem_instr]") as "mem_acc_tx".
 
-    iApply ("IH" $! _ _ (delete r1 trans) _ Htotal_regs' with "[] [] [] [] regs tx pgt_tx pgt_acc [own_tran excl_tran pgt_owned] [fresh_handles trans]
-                            [tran_pgt_transferred] [retri retri'] R0z R1z R2z rx_state rx other_rx prop0 propi [tran_pgt_owned]
+    iApply ("IH" $! _ _ (delete r1 trans) _ Htotal_rxs Htotal_regs' with "[] [] [] [] regs tx pgt_tx pgt_acc [own_tran excl_tran pgt_owned] [fresh_handles trans]
+                            [tran_pgt_transferred] [retri retri'] R0z R1z R2z rx rx_state other_rx prop0 propi [tran_pgt_owned]
                             [retri_owned] [mem_rest mem_acc_tx mem_tx]").
     {
       iPureIntro.
@@ -472,7 +474,7 @@ Lemma ftlr_reclaim {i mem_acc_tx ai regs ps_acc p_tx p_rx instr trans rx_state r
       rewrite /transaction_pagetable_entries_transferred.
       rewrite (big_sepFM_delete_False Hlookup_tran).
       iFrame "tran_pgt_transferred".
-      simpl. intros [? _]. rewrite Heq_tran_tt in H0; inversion H0.
+      simpl. intros [_ ?]. rewrite Heq_tran_tt in H0; inversion H0.
     }
     {
       rewrite /retrievable_transaction_transferred.
@@ -517,8 +519,8 @@ Lemma ftlr_reclaim {i mem_acc_tx ai regs ps_acc p_tx p_rx instr trans rx_state r
     iDestruct ("Hacc_regs" $! (ai ^+ 1)%f with "[$ PC $ R0 $ R1 $ R2]") as (regs') "[%Htotal_regs' regs]".
     iDestruct ("Hacc_mem_acc_tx" with "[$mem_instr]") as "mem_acc_tx".
 
-    iApply ("IH" $! _ _ (delete r1 trans) _ Htotal_regs' with "[] [] [] [] regs tx pgt_tx pgt_acc [oe_tran pgt_tran pgt_owned] [fresh_handles trans]
-                            [tran_pgt_transferred] [retri retri'] R0z R1z R2z rx_state rx other_rx prop0 propi [tran_pgt_owned]
+    iApply ("IH" $! _ _ (delete r1 trans) _ Htotal_rxs Htotal_regs' with "[] [] [] [] regs tx pgt_tx pgt_acc [oe_tran pgt_tran pgt_owned] [fresh_handles trans]
+                            [tran_pgt_transferred] [retri retri'] R0z R1z R2z rx rx_state other_rx prop0 propi [tran_pgt_owned]
                             [retri_owned] [mem_rest mem_acc_tx mem_tx]").
     {
       iPureIntro.
@@ -583,7 +585,7 @@ Lemma ftlr_reclaim {i mem_acc_tx ai regs ps_acc p_tx p_rx instr trans rx_state r
       rewrite /transaction_pagetable_entries_transferred.
       rewrite (big_sepFM_delete_False Hlookup_tran).
       iFrame "tran_pgt_transferred".
-      simpl. intros [? _]. rewrite Heq_tran_tt in H0; inversion H0.
+      simpl. intros [_ ?]. rewrite Heq_tran_tt in H0; inversion H0.
     }
     {
       rewrite /retrievable_transaction_transferred.
