theories/logrel/ftlr_retrieve.v
@@ -12,8 +12,9 @@ Section ftlr_retrieve.
   Context `{hypparams:!HypervisorParameters}.
   Context `{vmG: !gen_VMG Σ}.
 
-Lemma ftlr_retrieve {i mem_acc_tx ai regs ps_acc p_tx p_rx instr trans rx_state r0}:
+Lemma ftlr_retrieve {i mem_acc_tx ai regs rxs ps_acc p_tx p_rx instr trans r0}:
   base_extra.is_total_gmap regs ->
+  base_extra.is_total_gmap rxs ->
   {[p_tx; p_rx]} ⊆ ps_acc ->
   currently_accessible_in_trans_memory_pages i trans ⊆ ps_acc ∖ {[p_tx; p_rx]} ->
   p_rx ∉ ps_acc ∖ {[p_rx; p_tx]} ∪ accessible_in_trans_memory_pages i trans ->
@@ -28,7 +29,8 @@ Lemma ftlr_retrieve {i mem_acc_tx ai regs ps_acc p_tx p_rx instr trans rx_state 
   regs !! R0 = Some r0 ->
   decode_hvc_func r0 = Some Retrieve ->
   p_tx ≠ p_rx ->
-  ⊢ ▷ (∀ (a : gmap reg_name Addr) (a0 : gset PID) (a1 : gmap Addr transaction) (a2 : option (Addr * VMID)),
+  ⊢ ▷ (∀ (a : gmap reg_name Addr) (a0 : gset PID) (a1 : gmap Addr transaction) (a2 : gmap VMID (option (Addr * VMID))),
+              ⌜base_extra.is_total_gmap a2⌝ -∗
               ⌜base_extra.is_total_gmap a⌝ -∗
               ⌜{[p_tx; p_rx]} ⊆ a0⌝ -∗
               ⌜currently_accessible_in_trans_memory_pages i a1 ⊆ a0 ∖ {[p_tx; p_rx]}⌝ -∗
@@ -45,10 +47,10 @@ Lemma ftlr_retrieve {i mem_acc_tx ai regs ps_acc p_tx p_rx instr trans rx_state 
               R0 @@ V0 ->r encode_hvc_func Run -∗
               R1 @@ V0 ->r encode_vmid i -∗
               (∃ r2 : Addr, R2 @@ V0 ->r r2) -∗
-              RX_state@i:= a2 -∗
               mailbox.rx_page i p_rx -∗
-              rx_pages (list_to_set list_of_vmids ∖ {[i]}) -∗
-              ▷ VMProp V0 (vmprop_zero i p_tx p_rx) (1 / 2) -∗
+              rx_state_get i a2 -∗
+              rx_states_global (delete i a2) -∗
+              ▷ VMProp V0 (vmprop_zero i p_tx p_rx a2) (1 / 2) -∗
               VMProp i (vmprop_unknown i p_tx p_rx) 1 -∗
               transaction_pagetable_entries_owned i a1 -∗
               retrieved_transaction_owned i a1 -∗
@@ -65,10 +67,10 @@ Lemma ftlr_retrieve {i mem_acc_tx ai regs ps_acc p_tx p_rx instr trans rx_state 
    R0 @@ V0 ->r encode_hvc_func Run -∗
    R1 @@ V0 ->r encode_vmid i -∗
    (∃ r2 : Addr, R2 @@ V0 ->r r2) -∗
-   RX_state@i:= rx_state -∗
+   rx_state_get i rxs -∗
    mailbox.rx_page i p_rx -∗
-   rx_pages (list_to_set list_of_vmids ∖ {[i]}) -∗
-   ▷ VMProp V0 (vmprop_zero i p_tx p_rx) (1 / 2) -∗
+   rx_states_global (delete i rxs) -∗
+   ▷ VMProp V0 (vmprop_zero i p_tx p_rx rxs) (1 / 2) -∗
    VMProp i (vmprop_unknown i p_tx p_rx) 1 -∗
    transaction_pagetable_entries_owned i trans -∗
    retrieved_transaction_owned i trans -∗
@@ -77,9 +79,9 @@ Lemma ftlr_retrieve {i mem_acc_tx ai regs ps_acc p_tx p_rx instr trans rx_state 
    (∃ mem2 : mem, memory_page p_tx mem2) -∗
    SSWP ExecI @ i {{ bm, (if bm.1 then VMProp_holds i (1 / 2) else True) -∗ WP bm.2 @ i {{ _, True }} }}.
   Proof.
-    iIntros (Htotal_regs Hsubset_mb Hsubset_acc Hnin_rx Hnin_tx Hlookup_PC Hin_ps_acc Hneq_ptx Hdom_mem_acc_tx Hin_ps_acc_tx
-                         Hlookup_mem_ai Heqn Hlookup_reg_R0 Hdecode_hvc Hneq_mb).
-    iIntros  "IH regs tx pgt_tx pgt_acc pgt_owned trans_hpool_global tran_pgt_transferred retri R0z R1z R2z rx_state rx other_rx prop0
+    iIntros (Htotal_regs Htotal_rxs Hsubset_mb Hsubset_acc Hnin_rx Hnin_tx Hlookup_PC Hin_ps_acc Hneq_ptx Hdom_mem_acc_tx Hin_ps_acc_tx
+                         Hlookup_mem_ai Heqn Hlookup_reg_R0 Hdecode_hvc).
+    iIntros (Hneq_mb) "IH regs tx pgt_tx pgt_acc pgt_owned trans_hpool_global tran_pgt_transferred retri R0z R1z R2z rx_state rx other_rx prop0
              propi tran_pgt_owned retri_owned mem_rest mem_acc_tx mem_tx".
     set ps_mem_in_trans := accessible_in_trans_memory_pages i trans.
     pose proof (Htotal_regs R1) as[r1 Hlookup_reg_R1].
@@ -103,8 +105,8 @@ Lemma ftlr_retrieve {i mem_acc_tx ai regs ps_acc p_tx p_rx instr trans rx_state 
         iDestruct ("Hacc_regs" $! (ai ^+ 1)%f with "[$ PC $ R0 $ R1 $ R2]") as (regs') "[%Htotal_regs' regs]".
         iDestruct ("Hacc_mem_acc_tx" with "[$mem_instr]") as "mem_acc_tx".
 
-        iApply ("IH" $! _ _ trans _ Htotal_regs' with "[] [] [] [] regs tx pgt_tx pgt_acc pgt_owned [fresh_handles trans]
-                            tran_pgt_transferred retri R0z R1z R2z rx_state [$rx $pgt_rx] other_rx prop0 propi tran_pgt_owned
+        iApply ("IH" $! _ _ trans _ Htotal_rxs Htotal_regs' with "[] [] [] [] regs tx pgt_tx pgt_acc pgt_owned [fresh_handles trans]
+                            tran_pgt_transferred retri R0z R1z R2z [$rx $pgt_rx] rx_state other_rx prop0 propi tran_pgt_owned
                              retri_owned [mem_rest mem_acc_tx mem_tx]");auto.
         {
           iExists hpool. iSplitL "";auto. iFrame.
@@ -127,8 +129,8 @@ Lemma ftlr_retrieve {i mem_acc_tx ai regs ps_acc p_tx p_rx instr trans rx_state 
       iDestruct ("Hacc_regs" $! (ai ^+ 1)%f with "[$ PC $ R0 $ R1 $ R2]") as (regs') "[%Htotal_regs' regs]".
       iDestruct ("Hacc_mem_acc_tx" with "[$mem_instr]") as "mem_acc_tx".
 
-      iApply ("IH" $! _ _  trans _ Htotal_regs' with "[] [] [] [] regs tx pgt_tx pgt_acc pgt_owned [fresh_handles trans]
-                            tran_pgt_transferred retri R0z R1z R2z rx_state [$rx $pgt_rx] other_rx prop0 propi tran_pgt_owned
+      iApply ("IH" $! _ _  trans _ Htotal_rxs Htotal_regs' with "[] [] [] [] regs tx pgt_tx pgt_acc pgt_owned [fresh_handles trans]
+                            tran_pgt_transferred retri R0z R1z R2z [$rx $pgt_rx] rx_state other_rx prop0 propi tran_pgt_owned
                             retri_owned [mem_rest mem_acc_tx mem_tx]");auto.
       {
         iExists hpool. iSplitL "";auto. iFrame.
@@ -161,8 +163,8 @@ Lemma ftlr_retrieve {i mem_acc_tx ai regs ps_acc p_tx p_rx instr trans rx_state 
       iDestruct ("Hacc_regs" $! (ai ^+ 1)%f with "[$ PC $ R0 $ R1 $ R2]") as (regs') "[%Htotal_regs' regs]".
       iDestruct ("Hacc_mem_acc_tx" with "[$mem_instr]") as "mem_acc_tx".
 
-      iApply ("IH" $! _ _ trans _ Htotal_regs' with "[] [] [] [] regs tx pgt_tx pgt_acc pgt_owned [fresh_handles tran pgt_tran trans]
-                            tran_pgt_transferred retri R0z R1z R2z rx_state [$rx $pgt_rx] other_rx prop0 propi tran_pgt_owned
+      iApply ("IH" $! _ _ trans _ Htotal_rxs Htotal_regs' with "[] [] [] [] regs tx pgt_tx pgt_acc pgt_owned [fresh_handles tran pgt_tran trans]
+                            tran_pgt_transferred retri R0z R1z R2z [$rx $pgt_rx] rx_state other_rx prop0 propi tran_pgt_owned
                             retri_owned [mem_rest mem_acc_tx mem_tx]");auto.
       {
         iExists hpool.
@@ -181,8 +183,7 @@ Lemma ftlr_retrieve {i mem_acc_tx ai regs ps_acc p_tx p_rx instr trans rx_state 
     }
 
     iDestruct ("retri") as "[retri retri']".
-    iDestruct (big_sepFM_lookup_Some Hlookup_tran with "retri") as "[re retri]".
-    simpl;left;done.
+    iDestruct (big_sepFM_lookup_Some Hlookup_tran with "retri") as "[re retri]". right;done.
 
     destruct (tran.2) eqn:Heq_retri.
     { (* apply [mem_retrieve_retrieved] *)
@@ -195,8 +196,8 @@ Lemma ftlr_retrieve {i mem_acc_tx ai regs ps_acc p_tx p_rx instr trans rx_state 
      iDestruct ("Hacc_regs" $! (ai ^+ 1)%f with "[$ PC $ R0 $ R1 $ R2]") as (regs') "[%Htotal_regs' regs]".
      iDestruct ("Hacc_mem_acc_tx" with "[$mem_instr]") as "mem_acc_tx".
 
-     iApply ("IH" $! _ _ trans _ Htotal_regs' with "[] [] [] [] regs tx pgt_tx pgt_acc pgt_owned [fresh_handles tran pgt_tran trans]
-                            tran_pgt_transferred [re retri retri'] R0z R1z R2z rx_state [$rx $pgt_rx] other_rx prop0 propi tran_pgt_owned
+     iApply ("IH" $! _ _ trans _ Htotal_rxs Htotal_regs' with "[] [] [] [] regs tx pgt_tx pgt_acc pgt_owned [fresh_handles tran pgt_tran trans]
+                            tran_pgt_transferred [re retri retri'] R0z R1z R2z [$rx $pgt_rx] rx_state other_rx prop0 propi tran_pgt_owned
                             retri_owned [mem_rest mem_acc_tx mem_tx]");auto.
      {
        iExists hpool.
@@ -208,8 +209,7 @@ Lemma ftlr_retrieve {i mem_acc_tx ai regs ps_acc p_tx p_rx instr trans rx_state 
      }
      {
        rewrite /retrievable_transaction_transferred.
-       iDestruct (big_sepFM_delete_acc_True tran with "retri") as "retri".
-       simpl. left;done.
+       iDestruct (big_sepFM_delete_acc_True tran with "retri") as "retri". right;done.
        rewrite Heq_retri.
        iDestruct ("retri" with "re") as "retri".
        rewrite insert_id;auto.
@@ -230,18 +230,23 @@ Lemma ftlr_retrieve {i mem_acc_tx ai regs ps_acc p_tx p_rx instr trans rx_state 
     }
     rewrite Hrw_tran.
 
-    destruct (rx_state)  eqn: Heq_rxstate.
+
+    pose proof (Htotal_rxs i) as [rx_state Hlookup_rs].
+    iDestruct ("rx_state" $! rx_state with "[]") as "rx_state".
+    { iPureIntro. exact Hlookup_rs. }
+
+    destruct (rx_state) eqn: Heq_rxstate.
     { (* apply [mem_retrieve_rx_full] *)
      iDestruct (mem_big_sepM_split mem_acc_tx Hlookup_mem_ai with "mem_acc_tx") as "[mem_instr Hacc_mem_acc_tx]".
-     iApply (mem_retrieve_rx_full ai r1 with "[$PC $mem_instr $R0 $R1 $R2 $pgt_acc $tx $re $tran $rx_state]");auto.
-     iNext.
-     iIntros "(PC & mem_instr & R0 & R1 & R2 & pgt_acc & tx & re & tran & rx_state) _".
+     iApply (mem_retrieve_rx_full ai r1 with "[$PC $mem_instr $R0 $R1 $R2 $pgt_acc $tx $re $tran rx_state]").
+     done. done. done. done. exists p;reflexivity. iFrame.
+     iNext. iIntros "(PC & mem_instr & R0 & R1 & R2 & pgt_acc & tx & re & tran & rx_state) _".
 
      iDestruct ("Hacc_regs" $! (ai ^+ 1)%f with "[$ PC $ R0 $ R1 $ R2]") as (regs') "[%Htotal_regs' regs]".
      iDestruct ("Hacc_mem_acc_tx" with "[$mem_instr]") as "mem_acc_tx".
 
-     iApply ("IH" $! _ _ trans _ Htotal_regs' with "[] [] [] [] regs tx pgt_tx pgt_acc pgt_owned [fresh_handles tran pgt_tran trans]
-                            tran_pgt_transferred [re retri retri'] R0z R1z R2z rx_state [$rx $pgt_rx] other_rx prop0 propi tran_pgt_owned
+     iApply ("IH" $! _ _ trans _ Htotal_rxs Htotal_regs' with "[] [] [] [] regs tx pgt_tx pgt_acc pgt_owned [fresh_handles tran pgt_tran trans]
+                            tran_pgt_transferred [re retri retri'] R0z R1z R2z [$rx $pgt_rx] [rx_state] other_rx prop0 propi tran_pgt_owned
                             retri_owned [mem_rest mem_acc_tx mem_tx]");auto.
      {
        iExists hpool.
@@ -254,12 +259,17 @@ Lemma ftlr_retrieve {i mem_acc_tx ai regs ps_acc p_tx p_rx instr trans rx_state 
      }
      {
        rewrite /retrievable_transaction_transferred.
-       iDestruct (big_sepFM_delete_acc_True tran with "retri") as "retri".
-       simpl. left;done.
+       iDestruct (big_sepFM_delete_acc_True tran with "retri") as "retri". right;done.
        rewrite Heq_retri.
        iDestruct ("retri" with "re") as "retri".
        rewrite insert_id;auto.
        iFrame.
+     }
+     {
+       iIntros (?) "%Hlookup_rs'".
+       rewrite Hlookup_rs in Hlookup_rs'.
+       inversion Hlookup_rs'.
+       done.
      }
      {
        iDestruct (memory_pages_split_singleton' p_tx ps_acc with "[mem_acc_tx $mem_tx]") as "mem_acc". set_solver + Hsubset_mb.
@@ -312,8 +322,8 @@ Lemma ftlr_retrieve {i mem_acc_tx ai regs ps_acc p_tx p_rx instr trans rx_state 
     destruct (tran.1.2) eqn:Heq_tran_tt.
     { (* retrieve donate*)
       iDestruct (big_sepFM_lookup_Some Hlookup_tran with "tran_pgt_transferred") as "[[tran' oe_tran] tran_pgt_transferred]".
-      simpl. split;first done. left;done.
-      rewrite Hrw_tran; clear Hrw_tran. simpl.
+      simpl. split;last done. right;done.
+      rewrite Hrw_tran; clear Hrw_tran. 
       iDestruct (pgt_split_quarter with "[$oe_tran pgt_tran]") as "oe_tran".
       { case_bool_decide. iFrame. inversion H. }
       iDestruct (big_sepS_sep with "oe_tran") as "[own_tran excl_tran]".
@@ -346,9 +356,26 @@ Lemma ftlr_retrieve {i mem_acc_tx ai regs ps_acc p_tx p_rx instr trans rx_state 
         iDestruct ("Hacc_regs" $! (ai ^+ 1)%f with "[$ PC $ R0 $ R1 $ R2]") as (regs') "[%Htotal_regs' regs]".
         iDestruct ("Hacc_mem_acc_tx_rx" with "[$mem_instr]") as "mem_acc_tx_rx".
 
-        iApply ("IH" $! _ _ (delete r1 trans) _ Htotal_regs' with "[] [] [] [] regs tx pgt_tx pgt_acc [own_tran excl_tran pgt_owned] [fresh_handles trans]
-                            [tran_pgt_transferred] [retri retri'] R0z R1z R2z rx_state [$rx $pgt_rx] other_rx prop0 propi [tran_pgt_owned]
+        set rxs' := <[(i:VMID):= Some (wl, tran.1.1.1.1)]>rxs.
+
+        iApply ("IH" $! _ _ (delete r1 trans) rxs' with "[] [] [] [] [] [] regs tx pgt_tx pgt_acc [own_tran excl_tran pgt_owned] [fresh_handles trans]
+                            [tran_pgt_transferred] [retri retri'] R0z R1z R2z [$rx $pgt_rx] [rx_state] [other_rx] [prop0] propi [tran_pgt_owned]
                             [retri_owned] [mem_rest mem_acc_tx_rx mem_rx mem_tx]").
+        {
+          iPureIntro.
+          intro.
+          destruct (decide (k = i)).
+          {
+            exists (Some (wl, tran.1.1.1.1)).
+            rewrite /rxs'.
+            subst k. rewrite lookup_insert //.
+          }
+          specialize (Htotal_rxs k).
+          rewrite /rxs' lookup_insert_ne //.
+        }
+        {
+          done.
+        }
         {
           iPureIntro.
           set_solver + Hsubset_mb.
@@ -425,6 +452,22 @@ Lemma ftlr_retrieve {i mem_acc_tx ai regs ps_acc p_tx p_rx instr trans rx_state 
           iFrame "retri retri'".
         }
         {
+          iIntros (?) "%Hlookup_rs'".
+          rewrite lookup_insert in Hlookup_rs'.
+          inversion Hlookup_rs'.
+          done.
+        }
+        {
+          rewrite /rx_states_global.
+          replace (delete i rxs) with (delete i rxs'). done.
+          rewrite /rxs' delete_insert_delete //.
+        }
+        {
+          rewrite vmprop_zero_equiv_rxs.
+          iNext. iExact "prop0".
+          rewrite /rxs' delete_insert_delete //.
+        }
+        {
           rewrite /transaction_pagetable_entries_owned.
           rewrite (big_sepFM_delete_False Hlookup_tran).
           iFrame "tran_pgt_owned".
@@ -473,9 +516,26 @@ Lemma ftlr_retrieve {i mem_acc_tx ai regs ps_acc p_tx p_rx instr trans rx_state 
 
         iDestruct ("Hacc_regs" $! (ai ^+ 1)%f with "[$ PC $ R0 $ R1 $ R2]") as (regs') "[%Htotal_regs' regs]".
 
-        iApply ("IH" $! _ _ (delete r1 trans) _ Htotal_regs' with "[] [] [] [] regs tx pgt_tx pgt_acc [own_tran excl_tran pgt_owned] [fresh_handles trans]
-                            [tran_pgt_transferred] [retri retri'] R0z R1z R2z rx_state [$rx $pgt_rx] other_rx prop0 propi [tran_pgt_owned]
+        set rxs' := <[(i:VMID):= Some (wl, tran.1.1.1.1)]>rxs.
+
+        iApply ("IH" $! _ _ (delete r1 trans) rxs' with "[] [] [] [] [] [] regs tx pgt_tx pgt_acc [own_tran excl_tran pgt_owned] [fresh_handles trans]
+                            [tran_pgt_transferred] [retri retri'] R0z R1z R2z [$rx $pgt_rx] [rx_state] [other_rx] [prop0] propi [tran_pgt_owned]
                             [retri_owned] [mem_rest mem_acc_tx_rx mem_rx mem_tx]").
+        {
+          iPureIntro.
+          intro.
+          destruct (decide (k = i)).
+          {
+            exists (Some (wl, tran.1.1.1.1)).
+            rewrite /rxs'.
+            subst k. rewrite lookup_insert //.
+          }
+          specialize (Htotal_rxs k).
+          rewrite /rxs' lookup_insert_ne //.
+        }
+        {
+          done.
+        }
         {
           iPureIntro.
           set_solver + Hsubset_mb.
@@ -553,6 +613,22 @@ Lemma ftlr_retrieve {i mem_acc_tx ai regs ps_acc p_tx p_rx instr trans rx_state 
           iFrame "retri retri'".
         }
         {
+          iIntros (?) "%Hlookup_rs'".
+          rewrite lookup_insert in Hlookup_rs'.
+          inversion Hlookup_rs'.
+          done.
+        }
+        {
+          rewrite /rx_states_global.
+          replace (delete i rxs) with (delete i rxs'). done.
+          rewrite /rxs' delete_insert_delete //.
+        }
+        {
+          rewrite vmprop_zero_equiv_rxs.
+          iNext. iExact "prop0".
+          rewrite /rxs' delete_insert_delete //.
+        }
+        {
           rewrite /transaction_pagetable_entries_owned.
           rewrite (big_sepFM_delete_False Hlookup_tran).
           iFrame "tran_pgt_owned".
@@ -606,9 +682,26 @@ Lemma ftlr_retrieve {i mem_acc_tx ai regs ps_acc p_tx p_rx instr trans rx_state 
         iDestruct ("Hacc_mem_acc_tx_rx" with "[$mem_instr]") as "mem_acc_tx_rx".
         iDestruct (retri_split with "re") as "[re re']".
 
-        iApply ("IH" $! _ _ (<[r1 := ((tran.1, true):transaction)]> trans) _ Htotal_regs' with "[] [] [] [] regs tx pgt_tx pgt_acc [pgt_owned]
-                            [fresh_handles trans tran pgt_tran] [tran_pgt_transferred] [retri retri' re] R0z R1z R2z rx_state [$rx $pgt_rx]
-                            other_rx prop0 propi [tran_pgt_owned] [retri_owned re' tran''] [mem_rest mem_acc_tx_rx mem_rx mem_tx]").
+        set rxs' := <[(i:VMID):= Some (wl, tran.1.1.1.1)]>rxs.
+
+        iApply ("IH" $! _ _ (<[r1 := ((tran.1, true):transaction)]> trans) rxs' with "[] [] [] [] [] [] regs tx pgt_tx pgt_acc [pgt_owned]
+                          [fresh_handles trans tran pgt_tran] [tran_pgt_transferred] [retri retri' re] R0z R1z R2z [$rx $pgt_rx] [rx_state]
+                          [other_rx] [prop0] propi [tran_pgt_owned] [retri_owned re' tran''] [mem_rest mem_acc_tx_rx mem_rx mem_tx]").
+        {
+          iPureIntro.
+          intro.
+          destruct (decide (k = i)).
+          {
+            exists (Some (wl, tran.1.1.1.1)).
+            rewrite /rxs'.
+            subst k. rewrite lookup_insert //.
+          }
+          specialize (Htotal_rxs k).
+          rewrite /rxs' lookup_insert_ne //.
+        }
+        {
+          done.
+        }
         {
           iPureIntro.
           set_solver + Hsubset_mb.
@@ -673,17 +766,33 @@ Lemma ftlr_retrieve {i mem_acc_tx ai regs ps_acc p_tx p_rx instr trans rx_state 
           rewrite /transaction_pagetable_entries_transferred.
           rewrite Hrw_tran /=.
           iApply (big_sepFM_update_False _ Hlookup_tran);auto.
-          simpl. rewrite Heq_tran_tt. intros [? _]. done.
-          simpl. intros [? _]. done.
+          rewrite Heq_tran_tt. intros [_ ?]. done.
+          intros [_ ?]. done.
         }
         {
           rewrite /retrievable_transaction_transferred.
           iDestruct (big_sepFM_delete_acc_True (tran.1, true) with "retri") as "retri".
-          simpl. left;done.
+          right;done.
           iDestruct (big_sepFM_delete_acc_False (tran.1, true) with "retri'") as "retri'".
           simpl. intro. destruct H;done.
           iDestruct ("retri" with "re") as "retri".
           iFrame.
+        }
+        {
+          iIntros (?) "%Hlookup_rs'".
+          rewrite lookup_insert in Hlookup_rs'.
+          inversion Hlookup_rs'.
+          done.
+        }
+        {
+          rewrite /rx_states_global.
+          replace (delete i rxs) with (delete i rxs'). done.
+          rewrite /rxs' delete_insert_delete //.
+        }
+        {
+          rewrite vmprop_zero_equiv_rxs.
+          iNext. iExact "prop0".
+          rewrite /rxs' delete_insert_delete //.
         }
         {
           rewrite /transaction_pagetable_entries_owned.
@@ -746,9 +855,25 @@ Lemma ftlr_retrieve {i mem_acc_tx ai regs ps_acc p_tx p_rx instr trans rx_state 
         iDestruct ("Hacc_regs" $! (ai ^+ 1)%f with "[$ PC $ R0 $ R1 $ R2]") as (regs') "[%Htotal_regs' regs]".
         iDestruct (retri_split with "re") as "[re re']".
 
-        iApply ("IH" $! _ _ (<[r1 := ((tran.1, true):transaction)]> trans) _ Htotal_regs' with "[] [] [] [] regs tx pgt_tx pgt_acc [pgt_owned]
-                            [fresh_handles trans tran pgt_tran] [tran_pgt_transferred] [retri retri' re] R0z R1z R2z rx_state [$rx $pgt_rx] other_rx
-                            prop0 propi [tran_pgt_owned] [retri_owned re' tran''] [mem_rest mem_acc_tx_rx mem_rx mem_tx]").
+        set rxs' := <[(i:VMID):= Some (wl, tran.1.1.1.1)]>rxs.
+        iApply ("IH" $! _ _ (<[r1 := ((tran.1, true):transaction)]> trans) rxs' with "[] [] [] [] [] [] regs tx pgt_tx pgt_acc [pgt_owned]
+                          [fresh_handles trans tran pgt_tran] [tran_pgt_transferred] [retri retri' re] R0z R1z R2z [$rx $pgt_rx] [rx_state]
+                          [other_rx] [prop0] propi [tran_pgt_owned] [retri_owned re' tran''] [mem_rest mem_acc_tx_rx mem_rx mem_tx]").
+        {
+          iPureIntro.
+          intro.
+          destruct (decide (k = i)).
+          {
+            exists (Some (wl, tran.1.1.1.1)).
+            rewrite /rxs'.
+            subst k. rewrite lookup_insert //.
+          }
+          specialize (Htotal_rxs k).
+          rewrite /rxs' lookup_insert_ne //.
+        }
+        {
+          done.
+        }
         {
           iPureIntro.
           set_solver + Hsubset_mb.
@@ -812,17 +937,33 @@ Lemma ftlr_retrieve {i mem_acc_tx ai regs ps_acc p_tx p_rx instr trans rx_state 
           rewrite /transaction_pagetable_entries_transferred.
           rewrite Hrw_tran /=.
           iApply (big_sepFM_update_False _ Hlookup_tran);auto.
-          simpl. rewrite Heq_tran_tt. intros [? _]. done.
-          simpl. intros [? _]. done.
+          rewrite Heq_tran_tt. intros [_ ?]. done.
+          intros [_ ?]. done.
         }
         {
           rewrite /retrievable_transaction_transferred.
           iDestruct (big_sepFM_delete_acc_True (tran.1, true) with "retri") as "retri".
-          simpl. left;done.
+          right;done.
           iDestruct (big_sepFM_delete_acc_False (tran.1, true) with "retri'") as "retri'".
-          simpl. intro. destruct H;done.
+          intro. destruct H;done.
           iDestruct ("retri" with "re") as "retri".
           iFrame.
+        }
+        {
+          iIntros (?) "%Hlookup_rs'".
+          rewrite lookup_insert in Hlookup_rs'.
+          inversion Hlookup_rs'.
+          done.
+        }
+        {
+          rewrite /rx_states_global.
+          replace (delete i rxs) with (delete i rxs'). done.
+          rewrite /rxs' delete_insert_delete //.
+        }
+        {
+          rewrite vmprop_zero_equiv_rxs.
+          iNext. iExact "prop0".
+          rewrite /rxs' delete_insert_delete //.
         }
         {
           rewrite /transaction_pagetable_entries_owned.
@@ -890,10 +1031,26 @@ Lemma ftlr_retrieve {i mem_acc_tx ai regs ps_acc p_tx p_rx instr trans rx_state 
         iDestruct ("Hacc_mem_acc_tx_rx" with "[$mem_instr]") as "mem_acc_tx_rx".
         iDestruct (retri_split with "re") as "[re re']".
 
-        iApply ("IH" $! _ _ (<[r1 := ((tran.1, true):transaction)]> trans) _ Htotal_regs' with "[] [] [] [] regs tx pgt_tx pgt_acc
-                            [pgt_owned] [fresh_handles trans tran pgt_tran]
-                            [tran_pgt_transferred] [retri retri' re] R0z R1z R2z rx_state [$rx $pgt_rx] other_rx prop0 propi [tran_pgt_owned]
-                            [retri_owned re' tran''] [mem_rest mem_acc_tx_rx mem_rx mem_tx]").
+        set rxs' := <[(i:VMID):= Some (wl, tran.1.1.1.1)]>rxs.
+
+        iApply ("IH" $! _ _ (<[r1 := ((tran.1, true):transaction)]> trans) rxs' with "[] [] [] [] [] [] regs tx pgt_tx pgt_acc [pgt_owned]
+                          [fresh_handles trans tran pgt_tran] [tran_pgt_transferred] [retri retri' re] R0z R1z R2z [$rx $pgt_rx] [rx_state]
+                          [other_rx] [prop0] propi [tran_pgt_owned] [retri_owned re' tran''] [mem_rest mem_acc_tx_rx mem_rx mem_tx]").
+        {
+          iPureIntro.
+          intro.
+          destruct (decide (k = i)).
+          {
+            exists (Some (wl, tran.1.1.1.1)).
+            rewrite /rxs'.
+            subst k. rewrite lookup_insert //.
+          }
+          specialize (Htotal_rxs k).
+          rewrite /rxs' lookup_insert_ne //.
+        }
+        {
+          done.
+        }
         {
           iPureIntro.
           set_solver + Hsubset_mb.
@@ -956,17 +1113,33 @@ Lemma ftlr_retrieve {i mem_acc_tx ai regs ps_acc p_tx p_rx instr trans rx_state 
           rewrite /transaction_pagetable_entries_transferred.
           rewrite Hrw_tran /=.
           iApply (big_sepFM_update_False _ Hlookup_tran);auto.
-          simpl. rewrite Heq_tran_tt. intros [? _]. done.
-          simpl. intros [? _]. done.
+          rewrite Heq_tran_tt. intros [_ ?]. done.
+          intros [_ ?]. done.
         }
         {
           rewrite /retrievable_transaction_transferred.
           iDestruct (big_sepFM_delete_acc_True (tran.1, true) with "retri") as "retri".
-          simpl. left;done.
+          right;done.
           iDestruct (big_sepFM_delete_acc_False (tran.1, true) with "retri'") as "retri'".
           simpl. intro. destruct H;done.
           iDestruct ("retri" with "re") as "retri".
           iFrame.
+        }
+        {
+          iIntros (?) "%Hlookup_rs'".
+          rewrite lookup_insert in Hlookup_rs'.
+          inversion Hlookup_rs'.
+          done.
+        }
+        {
+          rewrite /rx_states_global.
+          replace (delete i rxs) with (delete i rxs'). done.
+          rewrite /rxs' delete_insert_delete //.
+        }
+        {
+          rewrite vmprop_zero_equiv_rxs.
+          iNext. iExact "prop0".
+          rewrite /rxs' delete_insert_delete //.
         }
         {
           rewrite /transaction_pagetable_entries_owned.
@@ -1036,9 +1209,25 @@ Lemma ftlr_retrieve {i mem_acc_tx ai regs ps_acc p_tx p_rx instr trans rx_state 
         iDestruct ("Hacc_regs" $! (ai ^+ 1)%f with "[$ PC $ R0 $ R1 $ R2]") as (regs') "[%Htotal_regs' regs]".
         iDestruct (retri_split with "re") as "[re re']".
 
-        iApply ("IH" $! _ _ (<[r1 := ((tran.1, true):transaction)]> trans) _ Htotal_regs' with "[] [] [] [] regs tx pgt_tx pgt_acc [pgt_owned]
-                            [fresh_handles trans tran pgt_tran] [tran_pgt_transferred] [retri retri' re] R0z R1z R2z rx_state [$rx $pgt_rx]
-                            other_rx prop0 propi [tran_pgt_owned] [retri_owned re' tran''] [mem_rest mem_acc_tx_rx mem_rx mem_tx]").
+        set rxs' := <[(i:VMID):= Some (wl, tran.1.1.1.1)]>rxs.
+        iApply ("IH" $! _ _ (<[r1 := ((tran.1, true):transaction)]> trans) rxs' with "[] [] [] [] [] [] regs tx pgt_tx pgt_acc [pgt_owned]
+                          [fresh_handles trans tran pgt_tran] [tran_pgt_transferred] [retri retri' re] R0z R1z R2z [$rx $pgt_rx] [rx_state]
+                          [other_rx] [prop0] propi [tran_pgt_owned] [retri_owned re' tran''] [mem_rest mem_acc_tx_rx mem_rx mem_tx]").
+        {
+          iPureIntro.
+          intro.
+          destruct (decide (k = i)).
+          {
+            exists (Some (wl, tran.1.1.1.1)).
+            rewrite /rxs'.
+            subst k. rewrite lookup_insert //.
+          }
+          specialize (Htotal_rxs k).
+          rewrite /rxs' lookup_insert_ne //.
+        }
+        {
+          done.
+        }
         {
           iPureIntro.
           set_solver + Hsubset_mb.
@@ -1102,17 +1291,33 @@ Lemma ftlr_retrieve {i mem_acc_tx ai regs ps_acc p_tx p_rx instr trans rx_state 
           rewrite /transaction_pagetable_entries_transferred.
           rewrite Hrw_tran /=.
           iApply (big_sepFM_update_False _ Hlookup_tran);auto.
-          simpl. rewrite Heq_tran_tt. intros [? _]. done.
-          simpl. intros [? _]. done.
+          rewrite Heq_tran_tt. intros [_ ?]. done.
+          intros [_ ?]. done.
         }
         {
           rewrite /retrievable_transaction_transferred.
           iDestruct (big_sepFM_delete_acc_True (tran.1, true) with "retri") as "retri".
-          simpl. left;done.
+          right;done.
           iDestruct (big_sepFM_delete_acc_False (tran.1, true) with "retri'") as "retri'".
-          simpl. intro. destruct H;done.
+          intro. destruct H;done.
           iDestruct ("retri" with "re") as "retri".
           iFrame.
+        }
+        {
+          iIntros (?) "%Hlookup_rs'".
+          rewrite lookup_insert in Hlookup_rs'.
+          inversion Hlookup_rs'.
+          done.
+        }
+        {
+          rewrite /rx_states_global.
+          replace (delete i rxs) with (delete i rxs'). done.
+          rewrite /rxs' delete_insert_delete //.
+        }
+        {
+          rewrite vmprop_zero_equiv_rxs.
+          iNext. iExact "prop0".
+          rewrite /rxs' delete_insert_delete //.
         }
         {
           rewrite /transaction_pagetable_entries_owned.
