theories/logrel/ftlr_share.v
@@ -12,8 +12,9 @@ Section ftlr_share.
   Context `{hypparams:!HypervisorParameters}.
   Context `{vmG: !gen_VMG Σ}.
 
-Lemma ftlr_share {i mem_acc_tx ai regs ps_acc p_tx p_rx instr trans rx_state r0}:
+Lemma ftlr_share {i mem_acc_tx ai regs rxs ps_acc p_tx p_rx instr trans r0}:
   base_extra.is_total_gmap regs ->
+  base_extra.is_total_gmap rxs ->
   {[p_tx; p_rx]} ⊆ ps_acc ->
   currently_accessible_in_trans_memory_pages i trans ⊆ ps_acc ∖ {[p_tx; p_rx]} ->
   p_rx ∉ ps_acc ∖ {[p_rx; p_tx]} ∪ accessible_in_trans_memory_pages i trans ->
@@ -28,7 +29,8 @@ Lemma ftlr_share {i mem_acc_tx ai regs ps_acc p_tx p_rx instr trans rx_state r0}
   regs !! R0 = Some r0 ->
   decode_hvc_func r0 = Some Share ->
   p_tx ≠ p_rx ->
-  ⊢ ▷ (∀ (a : gmap reg_name Addr) (a0 : gset PID) (a1 : gmap Addr transaction) (a2 : option (Addr * VMID)),
+  ⊢ ▷ (∀ (a : gmap reg_name Addr) (a0 : gset PID) (a1 : gmap Addr transaction) (a2 : gmap VMID (option (Addr * VMID))),
+              ⌜base_extra.is_total_gmap a2⌝ -∗
               ⌜base_extra.is_total_gmap a⌝ -∗
               ⌜{[p_tx; p_rx]} ⊆ a0⌝ -∗
               ⌜currently_accessible_in_trans_memory_pages i a1 ⊆ a0 ∖ {[p_tx; p_rx]}⌝ -∗
@@ -45,10 +47,10 @@ Lemma ftlr_share {i mem_acc_tx ai regs ps_acc p_tx p_rx instr trans rx_state r0}
               R0 @@ V0 ->r encode_hvc_func Run -∗
               R1 @@ V0 ->r encode_vmid i -∗
               (∃ r2 : Addr, R2 @@ V0 ->r r2) -∗
-              RX_state@i:= a2 -∗
               mailbox.rx_page i p_rx -∗
-              rx_pages (list_to_set list_of_vmids ∖ {[i]}) -∗
-              ▷ VMProp V0 (vmprop_zero i p_tx p_rx) (1 / 2) -∗
+              rx_state_get i a2 -∗
+              rx_states_global (delete i a2) -∗
+              ▷ VMProp V0 (vmprop_zero i p_tx p_rx a2) (1 / 2) -∗
               VMProp i (vmprop_unknown i p_tx p_rx) 1 -∗
               transaction_pagetable_entries_owned i a1 -∗
               retrieved_transaction_owned i a1 -∗
@@ -65,10 +67,10 @@ Lemma ftlr_share {i mem_acc_tx ai regs ps_acc p_tx p_rx instr trans rx_state r0}
    R0 @@ V0 ->r encode_hvc_func Run -∗
    R1 @@ V0 ->r encode_vmid i -∗
    (∃ r2 : Addr, R2 @@ V0 ->r r2) -∗
-   RX_state@i:= rx_state -∗
+   rx_state_get i rxs -∗
    mailbox.rx_page i p_rx -∗
-   rx_pages (list_to_set list_of_vmids ∖ {[i]}) -∗
-   ▷ VMProp V0 (vmprop_zero i p_tx p_rx) (1 / 2) -∗
+   rx_states_global (delete i rxs) -∗
+   ▷ VMProp V0 (vmprop_zero i p_tx p_rx rxs) (1 / 2) -∗
    VMProp i (vmprop_unknown i p_tx p_rx) 1 -∗
    transaction_pagetable_entries_owned i trans -∗
    retrieved_transaction_owned i trans -∗
@@ -77,9 +79,9 @@ Lemma ftlr_share {i mem_acc_tx ai regs ps_acc p_tx p_rx instr trans rx_state r0}
    (∃ mem2 : mem, memory_page p_tx mem2) -∗
    SSWP ExecI @ i {{ bm, (if bm.1 then VMProp_holds i (1 / 2) else True) -∗ WP bm.2 @ i {{ _, True }} }}.
   Proof.
-    iIntros (Htotal_regs Hsubset_mb Hsubset_acc Hnin_rx Hnin_tx Hlookup_PC Hin_ps_acc Hneq_ptx Hdom_mem_acc_tx Hin_ps_acc_tx
-                         Hlookup_mem_ai Heqn Hlookup_reg_R0 Hdecode_hvc Hneq_mb).
-    iIntros "IH regs tx pgt_tx pgt_acc pgt_owned trans_hpool_global tran_pgt_transferred retri R0z R1z R2z rx_state rx other_rx prop0
+    iIntros (Htotal_regs Htotal_rxs Hsubset_mb Hsubset_acc Hnin_rx Hnin_tx Hlookup_PC Hin_ps_acc Hneq_ptx Hdom_mem_acc_tx Hin_ps_acc_tx
+                         Hlookup_mem_ai Heqn Hlookup_reg_R0 Hdecode_hvc).
+    iIntros (Hneq_mb) "IH regs tx pgt_tx pgt_acc pgt_owned trans_hpool_global tran_pgt_transferred retri R0z R1z R2z rx_state rx other_rx prop0
              propi tran_pgt_owned retri_owned mem_rest mem_acc_tx mem_tx".
     set ps_mem_in_trans := accessible_in_trans_memory_pages i trans.
     pose proof (Htotal_regs R1) as[r1 Hlookup_reg_R1].
@@ -96,8 +98,8 @@ Lemma ftlr_share {i mem_acc_tx ai regs ps_acc p_tx p_rx instr trans rx_state r0}
       iDestruct ("Hacc_regs" $! (ai ^+ 1)%f with "[$ PC $ R0 $ R1 $ R2]") as (regs') "[%Htotal_regs' regs]".
 
       iDestruct ("Hacc_mem_acc_tx" with "[$mem_instr]") as "mem_acc_tx".
-      iApply ("IH" $!  _ ps_acc trans _ Htotal_regs' Hsubset_mb Hsubset_acc Hnin_rx Hnin_tx with "regs tx pgt_tx pgt_acc pgt_owned trans_hpool_global
-                            tran_pgt_transferred retri R0z R1z R2z rx_state rx other_rx prop0 propi tran_pgt_owned  retri_owned [mem_rest mem_acc_tx mem_tx] ").
+      iApply ("IH" $!  _ ps_acc trans _ Htotal_rxs Htotal_regs' Hsubset_mb Hsubset_acc Hnin_rx Hnin_tx with "regs tx pgt_tx pgt_acc pgt_owned trans_hpool_global
+                            tran_pgt_transferred retri R0z R1z R2z rx rx_state other_rx prop0 propi tran_pgt_owned  retri_owned [mem_rest mem_acc_tx mem_tx] ").
       {
         iDestruct (memory_pages_split_singleton' p_tx ps_acc with "[mem_acc_tx $mem_tx]") as "mem_acc". set_solver + Hsubset_mb.
         iExists mem_acc_tx;by iFrame "mem_acc_tx".
@@ -114,8 +116,8 @@ Lemma ftlr_share {i mem_acc_tx ai regs ps_acc p_tx p_rx instr trans rx_state r0}
       iDestruct ("Hacc_regs" $! (ai ^+ 1)%f with "[$ PC $ R0 $ R1 $ R2]") as (regs') "[%Htotal_regs' regs]".
 
       iDestruct ("Hacc_mem_acc_tx" with "[$mem_instr]") as "mem_acc_tx".
-      iApply ("IH" $! _ ps_acc trans _ Htotal_regs' Hsubset_mb Hsubset_acc Hnin_rx Hnin_tx with "regs tx pgt_tx pgt_acc pgt_owned trans_hpool_global
-                            tran_pgt_transferred retri R0z R1z R2z rx_state rx other_rx prop0 propi tran_pgt_owned retri_owned [mem_rest mem_acc_tx mem_tx] ").
+      iApply ("IH" $! _ ps_acc trans _ Htotal_rxs Htotal_regs' Hsubset_mb Hsubset_acc Hnin_rx Hnin_tx with "regs tx pgt_tx pgt_acc pgt_owned trans_hpool_global
+                            tran_pgt_transferred retri R0z R1z R2z rx rx_state other_rx prop0 propi tran_pgt_owned retri_owned [mem_rest mem_acc_tx mem_tx] ").
       {
         iDestruct (memory_pages_split_singleton' p_tx ps_acc with "[mem_acc_tx mem_tx]") as "mem_acc". set_solver + Hsubset_mb.
         iSplitL "mem_acc_tx".
@@ -134,8 +136,8 @@ Lemma ftlr_share {i mem_acc_tx ai regs ps_acc p_tx p_rx instr trans rx_state r0}
       iDestruct ("Hacc_regs" $! (ai ^+ 1)%f with "[$ PC $ R0 $ R1 $ R2]") as (regs') "[%Htotal_regs' regs]".
 
       iDestruct ("Hacc_mem_acc_tx" with "[$mem_instr]") as "mem_acc_tx".
-      iApply ("IH" $! _ ps_acc trans _ Htotal_regs' Hsubset_mb Hsubset_acc Hnin_rx Hnin_tx with "regs tx pgt_tx pgt_acc pgt_owned trans_hpool_global
-                            tran_pgt_transferred retri R0z R1z R2z rx_state rx other_rx prop0 propi tran_pgt_owned retri_owned [mem_rest mem_acc_tx mem_tx]").
+      iApply ("IH" $! _ ps_acc trans _ Htotal_rxs Htotal_regs' Hsubset_mb Hsubset_acc Hnin_rx Hnin_tx with "regs tx pgt_tx pgt_acc pgt_owned trans_hpool_global
+                            tran_pgt_transferred retri R0z R1z R2z rx rx_state other_rx prop0 propi tran_pgt_owned retri_owned [mem_rest mem_acc_tx mem_tx]").
       {
         iDestruct (memory_pages_split_singleton' p_tx ps_acc with "[mem_acc_tx mem_tx]") as "mem_acc". set_solver + Hsubset_mb.
         iSplitL "mem_acc_tx".
@@ -156,8 +158,8 @@ Lemma ftlr_share {i mem_acc_tx ai regs ps_acc p_tx p_rx instr trans rx_state r0}
       iDestruct ("Hacc_regs" $! (ai ^+ 1)%f with "[$ PC $ R0 $ R1 $ R2]") as (regs') "[%Htotal_regs' regs]".
       iDestruct ("Hacc_mem_acc_tx" with "[$mem_instr]") as "mem_acc_tx".
 
-      iApply ("IH" $! _ ps_acc trans _ Htotal_regs' Hsubset_mb Hsubset_acc Hnin_rx Hnin_tx with "regs tx pgt_tx pgt_acc pgt_owned trans_hpool_global
-                            tran_pgt_transferred retri R0z R1z R2z rx_state rx other_rx prop0 propi tran_pgt_owned retri_owned [mem_rest mem_acc_tx mem_tx]").
+      iApply ("IH" $! _ ps_acc trans _ Htotal_rxs Htotal_regs' Hsubset_mb Hsubset_acc Hnin_rx Hnin_tx with "regs tx pgt_tx pgt_acc pgt_owned trans_hpool_global
+                            tran_pgt_transferred retri R0z R1z R2z rx rx_state other_rx prop0 propi tran_pgt_owned retri_owned [mem_rest mem_acc_tx mem_tx]").
       {
         iDestruct (memory_pages_split_singleton' p_tx ps_acc with "[mem_acc_tx mem_tx]") as "mem_acc". set_solver + Hsubset_mb.
         iSplitL "mem_acc_tx".
@@ -176,8 +178,8 @@ Lemma ftlr_share {i mem_acc_tx ai regs ps_acc p_tx p_rx instr trans rx_state r0}
       iDestruct ("Hacc_regs" $! (ai ^+ 1)%f with "[$ PC $ R0 $ R1 $ R2]") as (regs') "[%Htotal_regs' regs]".
 
       iDestruct ("Hacc_mem_acc_tx" with "[$mem_instr]") as "mem_acc_tx".
-      iApply ("IH" $! _ ps_acc trans _ Htotal_regs' Hsubset_mb Hsubset_acc Hnin_rx Hnin_tx with "regs tx [$own_tx $excl_tx] pgt_acc pgt_owned trans_hpool_global
-                            tran_pgt_transferred retri R0z R1z R2z rx_state rx other_rx prop0 propi tran_pgt_owned retri_owned [mem_rest mem_acc_tx mem_tx]").
+      iApply ("IH" $! _ ps_acc trans _ Htotal_rxs Htotal_regs' Hsubset_mb Hsubset_acc Hnin_rx Hnin_tx with "regs tx [$own_tx $excl_tx] pgt_acc pgt_owned trans_hpool_global
+                            tran_pgt_transferred retri R0z R1z R2z rx rx_state other_rx prop0 propi tran_pgt_owned retri_owned [mem_rest mem_acc_tx mem_tx]").
       {
         iDestruct (memory_pages_split_singleton' p_tx ps_acc with "[mem_acc_tx mem_tx]") as "mem_acc". set_solver + Hsubset_mb.
         iSplitL "mem_acc_tx".
@@ -197,8 +199,8 @@ Lemma ftlr_share {i mem_acc_tx ai regs ps_acc p_tx p_rx instr trans rx_state r0}
       iDestruct ("Hacc_regs" $! (ai ^+ 1)%f with "[$ PC $ R0 $ R1 $ R2]") as (regs') "[%Htotal_regs' regs]".
 
       iDestruct ("Hacc_mem_acc_tx" with "[$mem_instr]") as "mem_acc_tx".
-      iApply ("IH" $! _ ps_acc trans _ Htotal_regs' Hsubset_mb Hsubset_acc Hnin_rx Hnin_tx with "regs tx pgt_tx pgt_acc pgt_owned trans_hpool_global
-                            tran_pgt_transferred retri R0z R1z R2z rx_state [$rx $own_rx $excl_rx] other_rx prop0 propi tran_pgt_owned retri_owned [mem_rest mem_acc_tx mem_tx]").
+      iApply ("IH" $! _ ps_acc trans _ Htotal_rxs Htotal_regs' Hsubset_mb Hsubset_acc Hnin_rx Hnin_tx with "regs tx pgt_tx pgt_acc pgt_owned trans_hpool_global
+                            tran_pgt_transferred retri R0z R1z R2z [$rx $own_rx $excl_rx] rx_state other_rx prop0 propi tran_pgt_owned retri_owned [mem_rest mem_acc_tx mem_tx]").
       {
         iDestruct (memory_pages_split_singleton' p_tx ps_acc with "[mem_acc_tx mem_tx]") as "mem_acc". set_solver + Hsubset_mb.
         iSplitL "mem_acc_tx".
@@ -242,8 +244,8 @@ Lemma ftlr_share {i mem_acc_tx ai regs ps_acc p_tx p_rx instr trans rx_state r0}
         iDestruct ("Hacc_regs" $! (ai ^+ 1)%f _ _ _ with "[$ PC $ R0 $ R1 $ R2]") as (regs') "[%Htotal_regs' regs]".
         iDestruct ("Hacc_mem_acc_tx" with "[$mem_instr]") as "mem_acc_tx".
 
-        iApply ("IH" $! _ ps_acc trans _ Htotal_regs' Hsubset_mb Hsubset_acc Hnin_rx Hnin_tx with "regs tx pgt_tx pgt_acc [pgt_owned] [fresh_handles trans]
-                            tran_pgt_transferred retri R0z R1z R2z rx_state rx other_rx prop0 propi tran_pgt_owned retri_owned [mem_rest mem_acc_tx mem_tx]").
+        iApply ("IH" $! _ ps_acc trans _ Htotal_rxs Htotal_regs' Hsubset_mb Hsubset_acc Hnin_rx Hnin_tx with "regs tx pgt_tx pgt_acc [pgt_owned] [fresh_handles trans]
+                            tran_pgt_transferred retri R0z R1z R2z rx rx_state other_rx prop0 propi tran_pgt_owned retri_owned [mem_rest mem_acc_tx mem_tx]").
         rewrite /pagetable_entries_excl_owned /pgt.
         iApply (big_sepS_subseteq with "pgt_owned").
         rewrite difference_union_L. set_solver +.
@@ -289,9 +291,9 @@ Lemma ftlr_share {i mem_acc_tx ai regs ps_acc p_tx p_rx instr trans rx_state r0}
       rewrite half_of_half.
       iDestruct (pgt_split_quarter with "pgt_oe_share") as "[pgt_oe_share_1 pgt_oe_share_3]".
 
-      iApply ("IH" $! _ ps_acc trans' _ Htotal_regs' Hsubset_mb with "[] [] [] regs tx pgt_tx pgt_acc [pgt_owned]
+      iApply ("IH" $! _ ps_acc trans' _ Htotal_rxs Htotal_regs' Hsubset_mb with "[] [] [] regs tx pgt_tx pgt_acc [pgt_owned]
                 [fresh_handles tran_share trans pgt_oe_share_3] [tran_pgt_transferred] [retri retri_share tran_share''] R0z R1z R2z
-                rx_state rx other_rx prop0 propi [tran_pgt_owned tran_share' pgt_oe_share_1] [retri_owned] [mem_rest mem_acc_tx mem_tx]").
+                rx rx_state other_rx prop0 propi [tran_pgt_owned tran_share' pgt_oe_share_1] [retri_owned] [mem_rest mem_acc_tx mem_tx]").
       {
         iPureIntro.
         rewrite /currently_accessible_in_trans_memory_pages /trans'.
@@ -346,7 +348,7 @@ Lemma ftlr_share {i mem_acc_tx ai regs ps_acc p_tx p_rx instr trans rx_state r0}
       {
         rewrite /transaction_pagetable_entries_transferred.
         iApply (big_sepFM_lookup_None_False with "tran_pgt_transferred"); auto.
-        simpl. intros [H _];inversion H.
+        simpl. intros [_ H];inversion H.
       }
       {
         rewrite /retrievable_transaction_transferred.
@@ -397,8 +399,8 @@ Lemma ftlr_share {i mem_acc_tx ai regs ps_acc p_tx p_rx instr trans rx_state r0}
       iDestruct ("Hacc_mem_acc_tx" with "[$mem_instr]") as "mem_acc_tx".
       iDestruct ("Hacc_trans" with "[$tran_tran $pgt]") as "trans".
 
-      iApply ("IH" $! _ ps_acc trans _ Htotal_regs' Hsubset_mb Hsubset_acc Hnin_rx Hnin_tx with "regs tx pgt_tx pgt_acc pgt_owned [fresh_handles trans]
-                            tran_pgt_transferred retri R0z R1z R2z rx_state rx other_rx prop0 propi tran_pgt_owned retri_owned [mem_rest mem_acc_tx mem_tx] ").
+      iApply ("IH" $! _ ps_acc trans _ Htotal_rxs Htotal_regs' Hsubset_mb Hsubset_acc Hnin_rx Hnin_tx with "regs tx pgt_tx pgt_acc pgt_owned [fresh_handles trans]
+                            tran_pgt_transferred retri R0z R1z R2z rx rx_state other_rx prop0 propi tran_pgt_owned retri_owned [mem_rest mem_acc_tx mem_tx] ").
       iExists hpool;by iFrame.
       {
         iDestruct (memory_pages_split_singleton' p_tx ps_acc with "[mem_acc_tx mem_tx]") as "mem_acc". set_solver + Hsubset_mb.
