theories/logrel/logrel_extra.v
@@ -1203,4 +1203,23 @@ Section logrel_extra.
     iPureIntro. rewrite map_union_assoc //. set_solver + Hneq_tx_rx.
   Qed.
 
+  Lemma vmprop_zero_equiv_rxs{p_tx p_rx} i rxs rxs' :
+  delete i rxs = delete i rxs' ->
+  VMProp V0 (vmprop_zero i p_tx p_rx rxs) (1 / 2) ⊣⊢
+  VMProp V0 (vmprop_zero i p_tx p_rx rxs') (1 / 2).
+  Proof.
+    intro.
+    rewrite /VMProp /=.
+    do 7 f_equiv.
+    rewrite /vmprop_zero.
+    rewrite /vmprop_zero_pre.
+    do 12 f_equiv.
+    rewrite /return_reg_rx.
+    do 4 f_equiv.
+    done.
+    do 12 f_equiv.
+    done.
+  Qed.
+
+
 End logrel_extra.
